split the definitions from the reduction function

original_work/TS_To_XC/TS_To_XC.thy
@@ -2,57 +2,86 @@ theory TS_To_XC
   imports TS_To_XC_aux
 begin
 
+definition vars_of_sat :: "'a three_sat \<Rightarrow> 'a xc_element set" where
+"vars_of_sat F = {V v |v. v \<in> vars F}"
+
+definition clauses_of_sat :: "'a three_sat \<Rightarrow> 'a xc_element set" where 
+"clauses_of_sat F = {C c| c. c\<in> set F}"
+
+definition literals_of_sat :: "'a three_sat \<Rightarrow> 'a xc_element set" where
+"literals_of_sat F = comp_literals F {}"
+
+definition literal_sets
+  :: "'a xc_element set \<Rightarrow> 'a xc_element set set" where
+"literal_sets Li = {{l}| l. l \<in> Li}"
+
+definition clauses_with_literals 
+  :: "'a xc_element set \<Rightarrow> 'a xc_element set \<Rightarrow> 'a xc_element set set" where
+"clauses_with_literals Cl Li = {{C c, l} |c l. C c \<in> Cl \<and> l \<in> Li 
+        \<and> l \<in> {L a c | a. a \<in> c}}"
+
+definition var_true_literals
+  :: "'a xc_element set \<Rightarrow> 'a xc_element set \<Rightarrow> 'a xc_element set 
+       \<Rightarrow> 'a xc_element set set" where 
+"var_true_literals Va Cl Li = 
+  {{V v} \<union> {l. l \<in> Li \<and> (\<exists>c. C c\<in> Cl \<and> L (Neg v) c = l)} |v. V v \<in> Va}"
+
+definition var_false_literals
+  :: "'a xc_element set \<Rightarrow> 'a xc_element set \<Rightarrow> 'a xc_element set 
+       \<Rightarrow> 'a xc_element set set" where 
+"var_false_literals Va Cl Li = 
+  {{V v} \<union> {l. l \<in> Li \<and> (\<exists>c. C c\<in> Cl \<and> L (Pos v) c = l)} |v. V v \<in> Va}"
+
 definition ts_xc :: "'a three_sat \<Rightarrow> 'a xc_element set * 'a xc_element set set" where 
-"ts_xc F = 
-  (if F \<in> three_cnf_sat 
-  then 
-  (let
-   vars = {V v |v. v \<in> vars F};
-   clauses = {C c| c. c\<in> set F};
-   literals = comp_literals F {};
-   literals_sets = {{l}| l. l \<in> literals};
-   clause_with_literal_sets = {{C c, l} |c l. C c \<in> clauses \<and> l \<in> literals 
-        \<and> l \<in> {L a c | a. a \<in> c}};
+"ts_xc F =(let
+   vars = vars_of_sat F;
+   clauses = clauses_of_sat F;
+   literals = literals_of_sat F;
+   literals_sets = literal_sets literals;
+   clause_with_literal_sets = clauses_with_literals clauses literals;
    var_true_sets = 
-    {{V v} \<union> {l. l \<in> literals \<and> (\<exists>c. C c\<in> clauses \<and> L (Neg v) c = l)} |v. V v \<in> vars};
+    var_true_literals vars clauses literals;
    var_false_sets = 
-    {{V v} \<union> {l. l \<in> literals \<and> (\<exists>c. C c\<in> clauses \<and> L (Pos v) c = l)} |v. V v \<in> vars}
+    var_false_literals vars clauses literals
   in
    (vars \<union> clauses \<union> literals,
-    literals_sets \<union> clause_with_literal_sets \<union> var_true_sets \<union> var_false_sets))
-  else ({}, {}))"
+    literals_sets \<union> clause_with_literal_sets \<union> var_true_sets \<union> var_false_sets))"
 
 lemma ts_xc_is_collection:
   assumes "ts_xc F = (X, S)" "F \<in> three_cnf_sat" 
   shows "\<Union>S \<subseteq> X"
-  proof -
-  let ?vars = "{V v |v. v \<in> vars F}"
-  let ?clauses = "{C c| c. c\<in> set F}"
-  let ?literals = "comp_literals F {}"
+proof -
+  let ?vars = "vars_of_sat F"
+  let ?clauses = "clauses_of_sat F"
+  let ?literals = "literals_of_sat F"
 
-  let ?ls = "{{l}| l. l \<in> ?literals}"
-  let ?cs = "{{C c, l} 
-    |c l. C c \<in> ?clauses \<and> l \<in> ?literals \<and> l \<in> {L a c | a. a \<in> c}}"
-  let ?vt = "{{V v} 
-   \<union> {l. l \<in> ?literals \<and> (\<exists>c. C c\<in> ?clauses \<and> L (Neg v) c = l)} |v. V v \<in> ?vars}"
-  let ?vf = " {{V v} 
-   \<union> {l. l \<in> ?literals \<and> (\<exists>c. C c\<in> ?clauses \<and> L (Pos v) c = l)} |v. V v \<in> ?vars}"
+  let ?ls = "literal_sets ?literals"
+  let ?cs = "clauses_with_literals ?clauses ?literals"
+  let ?vt = "var_true_literals ?vars ?clauses ?literals"
+  let ?vf = "var_false_literals ?vars ?clauses ?literals"
 
   have x_part: "X = ?vars \<union> ?clauses \<union> ?literals"
   using assms ts_xc_def[of F] by (auto simp: Let_def)
-   
+    
   have s_part: "S = ?ls \<union> ?cs \<union> ?vt \<union> ?vf"
   using assms ts_xc_def[of F] by (auto simp: Let_def)
 
-  have "\<Union>?ls = ?literals" by blast 
-  moreover have "\<Union>?cs \<subseteq> ?literals \<union> ?clauses" by blast
-  moreover have "\<Union>?vt \<subseteq> ?literals \<union> ?vars" by blast
-  moreover have "\<Union>?vf \<subseteq> ?literals \<union> ?vars" by blast
+  have "\<Union>?ls = ?literals" 
+    unfolding literal_sets_def by blast 
+
+  moreover have "\<Union>?cs \<subseteq> ?literals \<union> ?clauses" 
+    unfolding clauses_with_literals_def by blast
+
+  moreover have "\<Union>?vt \<subseteq> ?literals \<union> ?vars"
+    unfolding var_true_literals_def by blast
+    
+  moreover have "\<Union>?vf \<subseteq> ?literals \<union> ?vars" 
+    unfolding var_false_literals_def by blast
 
   ultimately have "\<Union> (?ls \<union> ?cs \<union> ?vt \<union> ?vf) \<subseteq> ?vars \<union> ?clauses \<union> ?literals"
   by blast
-  
+
   with x_part s_part show ?thesis by force
-  qed 
+qed 
 
 end
